spc/IPM.v
@@ -768,11 +768,8 @@ Section OWN.
     rewrite H0 in H. 
     esplits; et.
   Qed.
-
-  Tactic Notation "uiprop" := repeat (autounfold with iprop; autorewrite with iprop; s).
-  Tactic Notation "uiprop" "in" hyp(H)  := repeat (autounfold with iprop in H; autorewrite with iprop in H; simpl in H).
   
-  Lemma iProp_sepconj_aux P Q r 
+  (* Lemma iProp_sepconj_aux P Q r 
       (SAT: Own r ⊢ (P ** Q))
       (* (SAT: Own r ⊢ #=> (P ** Q)) *)
     :
@@ -842,6 +839,6 @@ Section OWN.
     eapply iProp_sepconj_aux in SAT; et. des.
     eapply Own_Upd in SAT.
     esplits; et. 	
-  Qed.	
+  Qed.	 *)
 
 End OWN.
